riscV/RelocProgSemanticsArchi1.v
@@ -1,0 +1,36 @@
+Require Import Coqlib Maps AST lib.Integers Values.
+Require Import Events lib.Floats Memory Smallstep.
+Require Import Asm RelocProg RelocProgram Globalenvs.
+Require Import Locations Stacklayout Conventions.
+Require Import Linking Errors.
+Require Import RelocProgSemantics Reloctablesgen.
+Require Import LocalLib.
+Import ListNotations.
+
+
+Definition rev_id_eliminate (symb: ident) (ofs : Z) (i:instruction) :=
+  match i with
+  | Pluil rd _ => Plui_s rd symb ofs
+  | Pluiw rd _ => Plui_s rd symb ofs
+  | Paddil rd rs _ => Paddi_s rd rs symb ofs
+  | Paddiw rd rs _ => Paddi_s rd rs symb ofs
+  | Pauipc rd (inr _) => Pauipc rd (inl symb)
+  | Pjal_ofs rd (inr _) => Pjal_ofs rd (inl symb)
+  | Plb  r1 r2 (Ofsimm _) => Plb  r1 r2  (Ofslow symb (Ptrofs.repr ofs))
+  | Plbu r1 r2 (Ofsimm _) => Plbu  r1 r2 (Ofslow symb (Ptrofs.repr ofs))
+  | Plh  r1 r2 (Ofsimm _) => Plh  r1 r2  (Ofslow symb (Ptrofs.repr ofs))
+  | Plhu r1 r2 (Ofsimm _) => Plhu  r1 r2 (Ofslow symb (Ptrofs.repr ofs))
+  | Plw  r1 r2 (Ofsimm _) => Plw  r1 r2  (Ofslow symb (Ptrofs.repr ofs))
+  | Pld  r1 r2 (Ofsimm _) => Pld  r1 r2  (Ofslow symb (Ptrofs.repr ofs))
+  | Pfls r1 r2 (Ofsimm _) => Pfls  r1 r2 (Ofslow symb (Ptrofs.repr ofs))
+  | Pfld r1 r2 (Ofsimm _) => Pfld  r1 r2 (Ofslow symb (Ptrofs.repr ofs))
+  | Psb  r1 r2 (Ofsimm _) => Psb  r1 r2  (Ofslow symb (Ptrofs.repr ofs))
+  | Psh  r1 r2 (Ofsimm _) => Psh  r1 r2  (Ofslow symb (Ptrofs.repr ofs))
+  | Psw  r1 r2 (Ofsimm _) => Psw  r1 r2  (Ofslow symb (Ptrofs.repr ofs))
+  | Psd  r1 r2 (Ofsimm _) => Psd  r1 r2  (Ofslow symb (Ptrofs.repr ofs))
+  | Pfss r1 r2 (Ofsimm _) => Pfss  r1 r2 (Ofslow symb (Ptrofs.repr ofs))
+  | Pfsd r1 r2 (Ofsimm _) => Pfsd  r1 r2 (Ofslow symb (Ptrofs.repr ofs))
+  | _ => i
+  end.
+ 
+ 
