riscV/ReloctablesgenSize.v
@@ -1,0 +1,50 @@
+Require Import Coqlib Maps Integers Floats Values AST Errors.
+Require Import Asm RelocProg RelocProgram.
+Require Import Hex compcert.encode.Bits Memdata Encode.
+Require Import LocalLib.
+Require Import ReloctablesgenArchi RelocProgSemanticsArchi1.
+Import Hex Bits.
+Import ListNotations.
+
+Local Open Scope error_monad_scope.
+Local Open Scope hex_scope.
+Local Open Scope bits_scope.
+
+
+Lemma rev_id_eliminate_size: forall i id addend, instr_size_real i = instr_size_real (rev_id_eliminate id addend i).
+Proof.
+  destruct i;intros;cbn;try destr;auto.
+Qed.
+
+Lemma id_eliminate_size_unchanged:forall i, instr_size_real i = instr_size_real (id_eliminate i).
+Proof.
+  destruct i;simpl;auto;try destr;auto.
+Qed.
+
+Section WITH_INSTR_SIZE.
+
+Variable instr_size : instruction -> Z.
+Hypothesis instr_size_bound : forall i, 0 < instr_size i <= Ptrofs.max_unsigned.
+
+Lemma transl_instr_range': forall ofs i e,
+    transl_instr instr_size ofs i = OK (Some e) ->
+    ofs <= e.(reloc_offset) < ofs + instr_size i.
+Proof.
+  intros ofs i e.
+  generalize (instr_size_bound i). intros A.
+  unfold transl_instr.
+  destruct i;intros H;inv H.
+  1-15: destr_match_in H11;inv H11;simpl;try lia.
+  1-2: simpl;lia.
+  destr_match_in H11. inv H11. simpl;lia.
+  inv H11.
+Qed.
+
+End WITH_INSTR_SIZE.
+
+Lemma transl_instr_range: forall ofs i e,
+    transl_instr instr_size_real ofs i = OK (Some e) ->
+    ofs <= e.(reloc_offset) < ofs + instr_size_real i.
+Proof.
+  eapply (transl_instr_range' instr_size_real instr_size_bound_real).
+Qed.
