riscV/ReloctablesgenproofArchi.v
@@ -1,0 +1,59 @@
+Require Import Coqlib Errors Maps.
+Require Import Integers Floats AST RelocProgLinking Linking.
+Require Import Op Locations Mach Conventions Asm RealAsm.
+Require Import Reloctablesgen ReloctablesgenArchi.
+Require Import RelocProg RelocProgram RelocProgSemantics RelocProgSemantics1 RelocProgGlobalenvs.
+Require Import Memory MemoryAgree.
+Require Import RelocProgSemanticsArchi RelocProgSemanticsArchi1.
+Require Import LocalLib AsmInject.
+Import ListNotations.
+
+Local Open Scope error_monad_scope.
+
+Section WITH_INSTR_SIZE.
+
+Variable instr_size : instruction -> Z.
+Hypothesis instr_size_bound : forall i, 0 < instr_size i <= Ptrofs.max_unsigned.
+
+
+Definition instr_eq (i1 i2: instruction) :=  i1=i2.
+
+Lemma instr_eq_refl: forall i, instr_eq i i.
+Proof.
+  unfold instr_eq.
+  auto.
+Qed.
+
+
+Lemma transl_instr_consistency: forall i ofs e,
+    transl_instr instr_size ofs i = OK (Some e) ->
+    instr_eq (rev_id_eliminate (reloc_symb e) (reloc_addend e) (id_eliminate i)) i.
+Proof.
+  intros.
+  unfold instr_eq. destruct i;simpl in *;auto;inv H.
+  1-15: destr_match_in H1;inv H1;simpl;try rewrite Ptrofs.repr_signed; auto.
+  1-2: destruct Archi.ptr64;simpl;auto.
+  destr_match_in H1;inv H1;simpl;try rewrite Ptrofs.repr_signed; auto.
+Qed.
+
+Lemma id_eliminate_unchanged:forall i ofs,
+    transl_instr instr_size ofs i = OK None ->
+    id_eliminate i = i.
+Proof.
+  intros i ofs.
+  destruct i;simpl;auto;
+  unfold transl_instr;simpl;intros;repeat (monadInv H);repeat (destr_in H);repeat monadInv H1.
+Qed.
+
+Lemma exec_instr_eq: forall (instr_size : instruction -> Z) (i i': instruction) (rs : regset) 
+                       (m : mem) (ge tge : Genv.t),
+    (forall (id : ident) (ofs : ptrofs), Genv.symbol_address ge id ofs = Genv.symbol_address tge id ofs) ->
+    instr_eq i' i ->
+    exec_instr instr_size ge i rs m = exec_instr instr_size tge i' rs m.
+Proof.
+  intros.
+  unfold instr_eq in H0.
+  destr_in H0;subst;try eapply exec_instr_refl;auto.
+Qed.
+
+End WITH_INSTR_SIZE.
