x86/ReloctablesgenproofArchi.v
@@ -2,11 +2,11 @@ Require Import Coqlib Errors Maps.
 Require Import Integers Floats AST RelocProgLinking Linking.
 Require Import Op Locations Mach Conventions Asm RealAsm.
 Require Import Reloctablesgen ReloctablesgenArchi.
-Require Import RelocProg RelocProgram RelocProgSemantics RelocProgSemantics1.
-Require Import RelocProgSemanticsArchi1.
+Require Import RelocProg RelocProgram RelocProgSemantics RelocProgSemantics1 RelocProgGlobalenvs.
+Require Import Memory MemoryAgree.
+Require Import RelocProgSemanticsArchi RelocProgSemanticsArchi1.
 Require Import LocalLib AsmInject.
 Import ListNotations.
-Require AsmFacts.
 
 Local Open Scope error_monad_scope.
 
@@ -14,14 +14,10 @@ Section WITH_INSTR_SIZE.
 
 Variable instr_size : instruction -> Z.
 Hypothesis instr_size_bound : forall i, 0 < instr_size i <= Ptrofs.max_unsigned.
-Hypothesis instr_reloc_bound : forall i ofs, instr_reloc_offset i = OK ofs -> 0 < ofs < instr_size i.
+
+(* unused 
 Hypothesis id_eliminate_size_unchanged:forall i, instr_size i = instr_size (id_eliminate i).
 
-Lemma lt_add_range:forall a b c,
-    0 < b < c -> a < a + b < a + c.
-Proof. 
-  intros. lia.
-Qed.
 
 Lemma code_id_eliminate_size_unchanged:forall c,
     code_size instr_size (transl_code' c) = code_size instr_size c.
@@ -30,95 +26,8 @@ Proof.
   induction c;simpl;auto.
   rewrite IHc. rewrite <- id_eliminate_size_unchanged.
   auto.
-Qed.
+Qed. *)
 
-Lemma transl_instr_range: forall ofs i e,
-    transl_instr instr_size ofs i = OK (Some e) ->
-    ofs < e.(reloc_offset) < ofs + instr_size i.
-  intros ofs i e.
-  generalize (instr_size_bound i). intros A.  
-  unfold transl_instr.
-
-  destruct Archi.ptr64 eqn:PTR.
-  -
-  (* 64bit *)
-  destruct i;intros H;destr_match_in H;try monadInv H. 
-  
-  (* only solve Pmov_rs *)  
-  unfold compute_instr_abs_relocentry in *. monadInv EQ0.
-  simpl;eapply lt_add_range; auto.
-
-  1-41: try (destruct a;destruct const;try destruct p;try monadInv H).
-  1-41: try (
-             unfold compute_instr_disp_relocentry in *;
-             try rewrite PTR in *;
-             unfold compute_instr_abs_relocentry in *;             
-             unfold compute_instr_rel_relocentry in *;
-             repeat (monadInv EQ0));
-  simpl;try eapply lt_add_range; auto.
-  
-  (* (* Pjmp_s *) *)
-  (* monadInv H1. *)
-  (* unfold compute_instr_rel_relocentry in *. *)
-  (* monadInv EQ. *)
-  (* destr_match_in EQ2;inv EQ2;simpl;eapply lt_add_range; auto. *)
-  (* inv H1. simpl. eapply lt_add_range; auto. *)
-  (* Pjmp_m *)
-  destruct base. monadInv H.
-  monadInv EQ0. 
-  simpl;eapply lt_add_range; auto.
-  destruct ofs0. monadInv H.
-  monadInv EQ0.
-  simpl;eapply lt_add_range; auto.
-  monadInv H. monadInv EQ0.
-  simpl. eapply lt_add_range; auto.
-  (* call_s *)
-  (* monadInv H1. unfold compute_instr_rel_relocentry in *. repeat (monadInv EQ). destr_match_in EQ2. inv EQ2. *)
-  (* simpl.  *)
-  (* eapply lt_add_range; auto. inv EQ2. *)
-  (* (* inv H1.   simpl.  *) *)
-  (* (* eapply lt_add_range; auto. *) *)
-  (* (* Pbuiltin *) *)
-  (* destr_match_in H1. *)
-  (* inv H1. inv H1. *)
-  (* Pmovw_rm *)
-  destruct ad;destruct const;try destruct p;monadInv H.
-  monadInv EQ0. simpl.
-  eapply lt_add_range; auto.
-  
-  (* 32 bit *)
-  -
-    destruct i;intros H;destr_match_in H;try monadInv H. 
-
-  (* only solve Pmov_rs *)  
-  unfold compute_instr_abs_relocentry in *. monadInv EQ0.
-  simpl;eapply lt_add_range; auto.
-            
-  1-41: try (destruct a;destruct const;try destruct p;try monadInv H).
-  1-41:try (
-             unfold compute_instr_disp_relocentry in *;
-             try rewrite PTR in *;
-             unfold compute_instr_abs_relocentry in *;             
-             unfold compute_instr_rel_relocentry in *;
-             repeat (monadInv EQ0));
-    simpl;try eapply lt_add_range; auto.
-  
- 
-  (* Pjmp_m *)
-  destruct base. monadInv H.
-  monadInv EQ0. 
-  simpl;eapply lt_add_range; auto.
-  destruct ofs0. monadInv H.
-  monadInv EQ0.
-  simpl;eapply lt_add_range; auto.
-  monadInv H. monadInv EQ0.
-  simpl;eapply lt_add_range; auto.
-
-  (* Pmovw_rm *)
-  destruct ad;destruct const;try destruct p;try monadInv H.
-  monadInv EQ0. simpl.
-  eapply lt_add_range; auto.
-Qed.
 
 (* id_eliminate just transforms Pjmp_s to Pjmp_l_rel and leaves another instruction forms unchanged *)
 Definition instr_eq i1 i2 :=
@@ -194,6 +103,18 @@ Proof.
   intros i ofs.
   destruct i;simpl;auto;
   unfold transl_instr;simpl;intros;repeat (monadInv H);repeat (destr_in H);repeat monadInv H1.
+Qed.
+
+Lemma exec_instr_eq: forall (instr_size : instruction -> Z) (i i': instruction) (rs : regset) 
+                       (m : mem) (ge tge : Genv.t),
+    (forall (id : ident) (ofs : ptrofs), Genv.symbol_address ge id ofs = Genv.symbol_address tge id ofs) ->
+    instr_eq i' i ->
+    exec_instr instr_size ge i rs m = exec_instr instr_size tge i' rs m.
+Proof.
+  intros.
+  unfold instr_eq in H0.
+  destr_in H0;subst;try eapply exec_instr_refl;auto.
+  destr_in H0;subst. simpl. rewrite H. auto.
 Qed.
 
 End WITH_INSTR_SIZE.
